bedrock2/src/bedrock2/Variables.v
@@ -8,6 +8,7 @@ Module expr. Import Syntax.expr.
     | literal v => nil
     | var x => cons x nil
     | load _ ea => vars ea
+    | inlinetable _ _ index => vars index
     | op _ e1 e2 => List.app (vars e1) (vars e2)
     end.
 End expr.
