compiler/src/compiler/FlatToRiscvLiterals.v
@@ -157,6 +157,7 @@ Section FlatToRiscvLiterals.
     - unfold compile_lit_64bit, compile_lit_32bit in *.
       remember (signExtend 12 (signExtend 32 (bitSlice v 32 64))) as mid.
       remember (signExtend 32 (signExtend 32 (bitSlice v 32 64))) as hi.
+      Simp.protect_equalities.
       cbv [List.app program array] in P.
       simpl in *. (* if you don't remember enough values, this might take forever *)
       repeat match type of X with
@@ -175,7 +176,7 @@ Section FlatToRiscvLiterals.
       rewrite E0.
       f_equal; [|simpl; try solve_MetricLog].
       f_equal.
-      + rewrite! map.put_put_same. f_equal. subst.
+      + rewrite! map.put_put_same. f_equal. Simp.unprotect_equalities. subst.
         apply word.unsigned_inj.
         assert (width = 64) as W64. {
           clear -E0.
